rupicola/io/LogRelTargetSource.CompatibilityLemmas.fst
@@ -650,13 +650,13 @@ let equiv_oprod_read_oval #g (fs_fd:fs_oval g qFileDescr) (fd:exp)
     (ensures fs_oprod_read_oval fs_fd ⊑ ERead fd)
   =
   lem_fv_in_env_read g fd;
-  introduce forall b (s:gsub g b) (fsG:eval_env g) (h:history). fsG `(≍) h` s ==> (qBool ^+ qUnit) ⫃ (h, read (fs_fd fsG), gsubst s (ERead fd)) with begin
+  introduce forall b (s:gsub g b) (fsG:eval_env g) (h:history). fsG `(≍) h` s ==> (qString ^+ qUnit) ⫃ (h, read (fs_fd fsG), gsubst s (ERead fd)) with begin
     let fs_fd = fs_fd fsG in
     let fs_e = read fs_fd in
     let e = ERead (gsubst s fd) in
     assert (gsubst s (ERead fd) == e);
     let ERead fd = e in
-    introduce fsG `(≍) h` s ==> (qBool ^+ qUnit) ⫃ (h, fs_e, e) with _. begin
+    introduce fsG `(≍) h` s ==> (qString ^+ qUnit) ⫃ (h, fs_e, e) with _. begin
       admit ()
     end
   end
